Bounded_Copy/Bounded_Copy_Convert.thy
@@ -5,148 +5,27 @@ theory Bounded_Copy_Convert
 begin
 
 
-lemma exist_only_list:
-  assumes "count_list w x = 1"
-  shows "\<exists>u v. (w = u @ x # v) \<and> (count_list u x = 0) \<and> (count_list v x = 0)"
-using assms proof (induct w)
-  case Nil
-  then show ?case by simp
+lemma "count_alpha (synthesize_shuffle_nat s) yk
+     = undefined"
+proof (cases yk rule: index_cases)
+  case (VarNone y)
+  then show ?thesis unfolding count_alpha_def synthesize_shuffle_nat_def
+    
+
 next
-  case (Cons a w)
-  then show ?case proof (cases "x = a")
-    case True
-    then show ?thesis using Cons.prems by (intro exI, auto)
-  next
-    case False
-    then show ?thesis proof -
-      have "count_list w x = 1" using Cons.prems False by simp
-      then obtain u v where uv: "(w = u @ x # v) \<and> (count_list u x = 0) \<and> (count_list v x = 0)"
-        using Cons.hyps by auto
-      have "a # w = (a # u) @ x # v \<and> (count_list u x = 0) \<and> (count_list v x = 0)" using uv by simp
-      then show ?thesis using False by fastforce
-    qed
-  qed
-qed
-
-lemma "set (concat (map f u)) = (\<Union>x\<in>set u. set (f x))"
-  by simp
-
-definition pred_only_x_y:
-  "pred_only_x_y x0 y0 yi = (\<forall>x y. (\<exists>k. yi = Inr (Inl (x, y, k))) \<longrightarrow> x = x0 \<and> y = y0)"
-
-lemma pred_only_x_y_apply: "pred_only_x_y x0 y0 (Inr (Inl (x, y, z))) \<longleftrightarrow> x = x0 \<and> y = y0"
-  unfolding pred_only_x_y by simp
-
-lemma synthesize_store_padding_x_y:
-  "list_all (pred_only_x_y x0 y0)
-     (concat
-       (map (synthesize_store B (Convert_Monoid_SST_Def.embed x0))
-            (padding B y0 xas)))"
-  unfolding synthesize_store_def pred_only_x_y 
-  by (induct xas rule: scanned_rev_induct, simp_all)
-
-lemma iota_x_y:
-  "list_all (pred_only_x_y x0 y0) (\<iota> B \<alpha> x0 y0)"
-  by (simp add: \<iota>_def synthesize_def synthesize_shuffle_def comp_def synthesize_store_padding_x_y)
-
-lemma y_neq_y0_count_list_zero: "y \<noteq> y0 \<Longrightarrow> count_list (\<iota> B \<alpha> x y) (Inr (Inl (x0, y0, z0))) = 0"
-proof -
-  assume y_neq_y0: "y \<noteq> y0"
-  have w: "\<forall>yi\<in>set (\<iota> B \<alpha> x y). pred_only_x_y x y yi"
-    by (simp add: iota_x_y Ball_set_list_all)
-  show ?thesis 
-    by (metis count_notin pred_only_x_y_apply w y_neq_y0)
+  case (VarSome y k)
+  then show ?thesis sorry
 qed
 
 
-lemma count_list_synthesize_ge_length:
-  assumes "length_scanned (scan u) \<le> enum_to_nat (z0 :: ('y::enum, 'k::enum) type_mult_suc)"
-  shows "count_list (concat (map (synthesize_store B (Convert_Monoid_SST_Def.embed x)) (padding B y (scan u))))
-                    (Inr (Inl (x0, y0, z0)))
-      = 0"
-using assms proof (induct u rule: xw_induct)
-  case (Word w)
-  then show ?case by (auto simp add: synthesize_store_def nat_enum_zero)
-next
-  case (VarWord x w u)
-  then show ?case proof (auto simp add: synthesize_store_def)
-    let ?enum = "Enum.enum :: ('y, 'k) type_mult_suc list"
-    have "enum_to_nat z0 < length ?enum" by (rule enum_nat_less)
-    then have "Suc (length_scanned (scan u)) < length ?enum"
-      using VarWord.prems by simp
-    then have "length_scanned (scan u) < length (Enum.enum :: ('y, 'k) type_mult_suc list)"
-      using Suc_lessD by blast
-    then have len: "enum_to_nat (nat_to_enum (length_scanned (scan u)) :: ('y, 'k) type_mult_suc) = length_scanned (scan u) "
-      by (simp add: nat_enum_iso)
-    assume "Suc (length_scanned (scan u)) \<le> enum_to_nat (nat_to_enum (length_scanned (scan u)) :: ('y, 'k) type_mult_suc)"
-    then show False using len by simp
-  qed
-qed
 
-lemma count_list_append: "count_list (xs @ ys) a = count_list xs a + count_list ys a"
-  by simp
-
-lemma map_Cons: "map f [x] = f x # map Inr []" by simp
-
-lemma count_list_synthesize_lt_length:
-  assumes "length_scanned (scan u) \<le> length (Enum.enum::('y::enum, 'k) type_mult_suc list)"
-  assumes "length_scanned (scan u) > enum_to_nat (z :: ('y::enum, 'k::enum) type_mult_suc)"
-  shows "count_list (concat (map (synthesize_store B (Convert_Monoid_SST_Def.embed x)) (padding B y (scan u))))
-                    (Inr (Inl (x, y, z)))
-       = 1"
-using assms proof (induct u rule: xw_induct)
-  case (Word w)
-  then show ?case by (simp add: synthesize_store_def nat_enum_zero enum_nat_zero_then_nat_enum_zero)
-next
-  case (VarWord x w u)
-  then show ?case proof (cases "enum_to_nat z = length_scanned (scan u)")
-    case True
-    then show ?thesis proof -
-      have *: "length_scanned (scan u) \<le> enum_to_nat z" using True by (simp add: )
-      have z: "z \<in> set (Enum.enum :: ('y, 'k) type_mult_suc list)" by (simp add: enum_UNIV)
-      thm count_list_synthesize_ge_length[OF *]
-      show ?thesis
-        apply (simp only: map_append scan_last_simp map_Cons padding_last_simp concat_append count_list_append)
-        apply (simp add: count_list_synthesize_ge_length[OF *])
-        apply (simp add: synthesize_store_def)
-        apply (simp add: True[symmetric] enum_nat_iso[OF z])
-        done
-    qed
-  next
-    case False
-    then show ?thesis using VarWord proof (simp add: synthesize_store_def)
-      let ?enum = "Enum.enum :: ('y, 'k) type_mult_suc list"
-      assume neq: "enum_to_nat z \<noteq> length_scanned (scan u)"
-      have "length_scanned (scan u) \<le> length ?enum" using VarWord.prems by simp
-      show "nat_to_enum (length_scanned (scan u)) \<noteq> z" proof (rule ccontr, simp)
-        assume "nat_to_enum (length_scanned (scan u)) = z"
-        then have "enum_to_nat (nat_to_enum (length_scanned (scan u)) :: ('y, 'k) type_mult_suc) = enum_to_nat z" by simp
-        moreover have condition: "length_scanned (scan u) < length ?enum" using VarWord.prems by simp
-        ultimately have "length_scanned (scan u) = enum_to_nat z" by (simp add: nat_enum_iso[OF condition])
-        then show False using neq by simp
-      qed
-    qed
-  qed
-qed
-
-lemma count_list_synthesize:
-  assumes "length_scanned (scan u) \<le> length (Enum.enum::('y::enum, 'k::enum) type_mult_suc list)"
-  shows "count_list (concat (map (synthesize_store B (Convert_Monoid_SST_Def.embed x)) (padding B y (scan u))))
-                    (Inr (Inl (x, y, z :: ('y, 'k) type_mult_suc))) \<le> Suc 0"
-proof (cases "length_scanned (scan u) \<le> enum_to_nat z")
-  case True
-  then show ?thesis by (simp add: count_list_synthesize_ge_length)
-next
-  case False
-  then show ?thesis by (simp add: count_list_synthesize_lt_length assms)
-qed
 
 lemma count_alpha_iota_le_1:
   fixes \<alpha> :: "'x \<Rightarrow> 'y::enum shuffle"
   assumes "boundedness (B :: 'k::enum boundedness) k"
   assumes "bounded_shuffle k (\<alpha> x)"
   shows "count_alpha (\<iota> B \<alpha> x :: ('y, 'x \<times> ('y, 'k::enum) index + 'b) update) (Inl (x0, y0, z0) :: 'x \<times> ('y, 'k::enum) index + 'b) \<le> 1"
-  sorry
+  unfolding \<iota>_def
 
 lemma count_alpha_iota_x_neq_x0_eq_0:
   fixes \<alpha> :: "'x \<Rightarrow> 'y::enum shuffle"
@@ -236,147 +115,6 @@ next
 qed
 
 
-theorem convert_MSST_bounded:
-  fixes msst :: "('q::finite, 'x::finite, 'y::enum, 'a, 'b) MSST"
-  fixes B2 :: "'l::enum boundedness"
-  assumes bc_msst: "bounded_copy_SST k msst"
-  assumes boundedness_k: "boundedness B1 k"
-  assumes boundedness_l: "boundedness B2 l"
-  assumes typed: "is_type msst \<gamma>"
-  assumes bc_type: "bounded_copy_type l msst \<gamma>"
-  shows "bounded_copy_SST (k * l) (convert_MSST B2 msst)"
-  unfolding bounded_copy_SST_def bounded_def
-proof (intro allI, rule impI)
-  fix w qb
-  assume "reachable (convert_MSST B2 msst) qb"
-  then have r_pair: "reachable (convert_MSST B2 msst) (fst qb, snd qb)" by simp
-  then have r_fst: "reachable msst (fst qb)" by (rule reachable_convert)
-  have l0: "0 < l" using assms length_enum_gt_0 unfolding boundedness_def by simp
-  have k0: "0 < k" using assms length_enum_gt_0 unfolding boundedness_def by simp
-
-  show "\<forall>y. count_var (SST.eta_hat (convert_MSST B2 msst) (qb, w)) y \<le> k * l"
-  proof (cases "length w")
-    case 0
-    then show ?thesis
-      apply simp unfolding count_var_def idU_def 
-      apply (simp only: sum_count_list_inj[OF inj_Inl])
-      apply (simp add: k0 l0 Suc_leI)
-      done
-  next
-    case (Suc nat)
-    then have w_gt_0: "0 < length w" by simp
-    note mado = convert_\<eta>_hat_gt_0[OF assms(3-5) r_pair w_gt_0, simplified]
-    then show ?thesis proof (auto simp add: mado count_var_def H'_def prod.case_eq_if)
-      fix x0 y0 z0
-      have "(\<Sum>xyz\<in>UNIV. count_list (resolve_store B2 (hat_homU (\<iota> B2 (Rep_alpha B2 (snd qb)))
-                                                                (SST.eta_hat msst (fst qb, w) (fst xyz))) (snd xyz))
-           (Inl (x0, y0, z0)))
-          = (\<Sum>(x, yk)\<in>UNIV. count_list (resolve_store B2 (hat_homU (\<iota> B2 (Rep_alpha B2 (snd qb))) (SST.eta_hat msst (fst qb, w) x)) yk)
-           (Inl (x0, y0, z0)))" (is "?lhs = _")
-        by (simp add: prod.case_eq_if)
-      also have "... = (\<Sum>x\<in>UNIV. \<Sum>yk\<in>UNIV. count_list (resolve_store B2 (hat_homU (\<iota> B2 (Rep_alpha B2 (snd qb))) (SST.eta_hat msst (fst qb, w) x)) yk)
-           (Inl (x0, y0, z0)))"
-        apply (simp only: UNIV_Times_UNIV[symmetric])
-        apply (rule sum.Sigma[symmetric], simp_all)
-        done
-      also have "... = (\<Sum>x\<in>UNIV. \<Sum>y\<in>UNIV. count_list (hat_homU (\<iota> B2 (Rep_alpha B2 (snd qb))) (SST.eta_hat msst (fst qb, w) x) y)
-           (Inr (Inl (x0, y0, z0))))"
-        by (simp add: sum_decompose[OF boundedness_l hat_homU_iota_bounded_copy[OF boundedness_l typed bc_type r_pair]])
-      also have "... = (\<Sum>x\<in>UNIV. count_alpha (hat_homU (\<iota> B2 (Rep_alpha B2 (snd qb))) (SST.eta_hat msst (fst qb, w) x)) (Inl (x0, y0, z0)))"
-        unfolding count_alpha_def by simp
-      also have "... \<le> k * l" proof -
-        have body: "\<And>x. count_alpha (hat_homU (\<iota> B2 (Rep_alpha B2 (snd qb))) (SST.eta_hat msst (fst qb, w) x)) (Inl (x0, y0, z0))
-                    \<le> count_list (SST.eta_hat msst (fst qb, w) x) (Inl x0) * l" proof -
-          fix x
-          have tail: "SST.eta_hat msst (fst qb, w) x \<in> tails (SST.eta_hat msst (fst qb, w) x)"
-            unfolding tails_def by auto
-          show "count_alpha (hat_homU (\<iota> B2 (Rep_alpha B2 (snd qb))) (SST.eta_hat msst (fst qb, w) x)) (Inl (x0, y0, z0))
-                    \<le> count_list (SST.eta_hat msst (fst qb, w) x) (Inl x0) * l"
-            by (simp add: count_alpha_hat_homU_eta_hat[OF bc_msst boundedness_l typed bc_type r_pair tail])
-        qed
-        have "(\<Sum>x\<in>UNIV. count_alpha (hat_homU (\<iota> B2 (Rep_alpha B2 (snd qb))) (SST.eta_hat msst (fst qb, w) x)) (Inl (x0, y0, z0)))
-            \<le> (\<Sum>x\<in>UNIV. count_list (SST.eta_hat msst (fst qb, w) x) (Inl x0) * l)"
-          by (simp add: body sum_mono)
-        also have "... = (\<Sum>x\<in>UNIV. count_list (SST.eta_hat msst (fst qb, w) x) (Inl x0)) * l"
-          by (metis (mono_tags, lifting) sum.cong sum_distrib_right)
-        also have "... = count_var (SST.eta_hat msst (fst qb, w)) x0 * l"
-          unfolding count_var_def by simp
-        also have "... \<le> k * l" proof -
-          have "bounded k (SST.eta_hat msst (fst qb, w))"
-            using bc_msst r_fst unfolding bounded_copy_SST_def by auto
-          then have "count_var (SST.eta_hat msst (fst qb, w)) x0 \<le> k"
-            by (simp add: bounded_def)
-          then show ?thesis by simp
-        qed
-        finally show ?thesis .
-      qed
-      finally show "?lhs \<le> k * l" .
-    qed
-  qed
-qed
-
-lemma count_list_in_set_distinct:
-  assumes "\<forall>a\<in>set xs. count_list xs a \<le> 1"
-  shows "distinct xs"
-  using assms proof (induct xs)
-case Nil
-  then show ?case by simp
-next
-  case (Cons x xs)
-  then show ?case proof (auto)
-    assume 0: "count_list xs x = 0"
-    moreover assume 1: "x \<in> set xs"
-    ultimately show False
-      using count_list_append split_list_last by force
-  next
-    assume xs_zero: "count_list xs x = 0"
-    have "\<forall>a\<in>set xs. count_list xs a \<le> Suc 0" proof
-      fix a
-      assume a: "a \<in> set xs"
-      then show "count_list xs a \<le> Suc 0" using xs_zero Cons.prems by (cases "a = x", auto)
-    qed
-    then show "distinct xs" using Cons.hyps by simp
-  qed
-qed
-
-lemma count_list_distinct:
-  assumes "\<forall>a. count_list xs a \<le> 1"
-  shows "distinct xs"
-  using assms by (simp add: count_list_in_set_distinct)
-
-
-
-lemma lookup_rec_all_not_in:
-  assumes "distinct ys"
-  assumes "\<forall>y0 \<in> set ys.   
-           Inr (x0, Some k0) \<notin> set (give_index_row (resolve_shuffle m)
-                                           (seek y0 ys) (resolve_shuffle m y0))"
-  shows "lookup_rec m x0 k0 ys = None"
-proof (cases ys)
-  case Nil
-  then show ?thesis using assms by simp
-next
-  case (Cons a list)
-  then obtain y0 where
-    y0: "y0 \<in> set ys \<and> lookup_rec m x0 k0 ys = lookup_row (resolve_shuffle m) x0 k0 (seek y0 ys) (scan_pair (m y0))"
-    using assms(1) lookup_rec_distinct by fast
-  then show ?thesis
-    apply (simp add: y0)
-    apply (rule there_doesnt_exist_corresponding_string)
-    using assms(2)
-    apply (simp add: y0)
-    done
-qed
-
-
-
-lemma 
-  assumes "distinct ys"
-  assumes "Inr (x0, Some k0) \<notin> 
-                 (\<Union>y0\<in>set ys. set (give_index_row (resolve_shuffle m)
-                                      (seek y0 ys) (resolve_shuffle m y0)))"
-  shows "lookup_rec m x0 k0 ys = None"
-  using assms by (simp add: lookup_rec_all_not_in)
 
 
 definition iterate_range :: "'k::enum boundedness \<Rightarrow> ('y::enum \<times> nat option) set"  where
@@ -623,6 +361,8 @@ proof -
   then show ?thesis by (simp add: compS_apply)
 qed
 
+lemma count_list_valuate: "count_list (valuate u) a = count_list u (Inr a)"
+  by (induct u rule: xa_induct, simp_all)
 
 lemma sum_decompose:
   fixes m :: "('y::enum, 'b) update"
@@ -630,7 +370,7 @@ lemma sum_decompose:
   assumes "boundedness B K"
   assumes "bounded K m"
   shows "(\<Sum>yk\<in>UNIV. count_list (resolve_store B m yk) a)
-       = (\<Sum>y\<in>UNIV. count_list (valuate (m y)) a)" (is "?from = ?to")
+       = (\<Sum>y\<in>UNIV. count_list (m y) (Inr a))" (is "?from = ?to")
 proof -
   let ?vars = "\<lambda>y. valuate (synthesize_shuffle_nat (resolve_shuffle m) y)"
   let ?resolve = "\<lambda>xk. resolve_store_nat m xk"
@@ -647,10 +387,97 @@ proof -
   also have "... = (\<Sum>y\<in>UNIV. count_list (concat (map ?resolve (?vars y))) a)"
     by (simp add: count_list_sum_list_concat_map)
   also have "... = ?to"
-    using resolve_inverse_nat_valuate by (simp add: compS_apply resolve_inverse_nat_valuate)
+    using resolve_inverse_nat_valuate by (simp add: compS_apply resolve_inverse_nat_valuate count_list_valuate)
   finally show ?thesis .
 qed
 
+
+theorem convert_MSST_bounded:
+  fixes msst :: "('q::finite, 'x::finite, 'y::enum, 'a, 'b) MSST"
+  fixes B1 :: "'k::enum boundedness"
+  fixes B2 :: "'l::enum boundedness"
+  assumes bc_msst: "bounded_copy_SST k msst"
+  assumes boundedness_k: "boundedness B1 k"
+  assumes boundedness_l: "boundedness B2 l"
+  assumes typed: "is_type msst \<gamma>"
+  assumes bc_type: "bounded_copy_type l msst \<gamma>"
+  shows "bounded_copy_SST (k * l) (convert_MSST B2 msst)"
+  unfolding bounded_copy_SST_def bounded_def
+proof (intro allI, rule impI)
+  fix w qb
+  assume "reachable (convert_MSST B2 msst) qb"
+  then have r_pair: "reachable (convert_MSST B2 msst) (fst qb, snd qb)" by simp
+  then have r_fst: "reachable msst (fst qb)" by (rule reachable_convert)
+  have l0: "0 < l" using assms length_enum_gt_0 unfolding boundedness_def by simp
+  have k0: "0 < k" using assms length_enum_gt_0 unfolding boundedness_def by simp
+
+  show "\<forall>y. count_var (SST.eta_hat (convert_MSST B2 msst) (qb, w)) y \<le> k * l"
+  proof (cases "length w")
+    case 0
+    then show ?thesis
+      apply simp unfolding count_var_def idU_def 
+      apply (simp only: sum_count_list_inj[OF inj_Inl])
+      apply (simp add: k0 l0 Suc_leI)
+      done
+  next
+    case (Suc nat)
+    then have w_gt_0: "0 < length w" by simp
+    note mado = convert_\<eta>_hat_gt_0[OF assms(3-5) r_pair w_gt_0, simplified]
+    then show ?thesis proof (auto simp add: mado count_var_def H'_def prod.case_eq_if)
+      fix x0 y0 z0
+      have "(\<Sum>xyz\<in>UNIV. count_list (resolve_store B2 (hat_homU (\<iota> B2 (Rep_alpha B2 (snd qb)))
+                                                                (SST.eta_hat msst (fst qb, w) (fst xyz))) (snd xyz))
+           (Inl (x0, y0, z0)))
+          = (\<Sum>(x, yk)\<in>UNIV. count_list (resolve_store B2 (hat_homU (\<iota> B2 (Rep_alpha B2 (snd qb))) (SST.eta_hat msst (fst qb, w) x)) yk)
+           (Inl (x0, y0, z0)))" (is "?lhs = _")
+        by (simp add: prod.case_eq_if)
+      also have "... = (\<Sum>x\<in>UNIV. \<Sum>yk\<in>UNIV. count_list (resolve_store B2 (hat_homU (\<iota> B2 (Rep_alpha B2 (snd qb))) (SST.eta_hat msst (fst qb, w) x)) yk)
+           (Inl (x0, y0, z0)))"
+        apply (simp only: UNIV_Times_UNIV[symmetric])
+        apply (rule sum.Sigma[symmetric], simp_all)
+        done
+      also have "... = (\<Sum>x\<in>UNIV. \<Sum>y\<in>UNIV. count_list (hat_homU (\<iota> B2 (Rep_alpha B2 (snd qb))) (SST.eta_hat msst (fst qb, w) x) y)
+           (Inr (Inl (x0, y0, z0))))"
+        by (simp add: sum_decompose[OF boundedness_l hat_homU_iota_bounded_copy[OF boundedness_l typed bc_type r_pair]])
+      also have "... = (\<Sum>x\<in>UNIV. count_alpha (hat_homU (\<iota> B2 (Rep_alpha B2 (snd qb))) (SST.eta_hat msst (fst qb, w) x)) (Inl (x0, y0, z0)))"
+        unfolding count_alpha_def by simp
+      also have "... \<le> k * l" proof -
+        have body: "\<And>x. count_alpha (hat_homU (\<iota> B2 (Rep_alpha B2 (snd qb))) (SST.eta_hat msst (fst qb, w) x)) (Inl (x0, y0, z0))
+                    \<le> count_list (SST.eta_hat msst (fst qb, w) x) (Inl x0) * l" proof -
+          fix x
+          have tail: "SST.eta_hat msst (fst qb, w) x \<in> tails (SST.eta_hat msst (fst qb, w) x)"
+            unfolding tails_def by auto
+          show "count_alpha (hat_homU (\<iota> B2 (Rep_alpha B2 (snd qb))) (SST.eta_hat msst (fst qb, w) x)) (Inl (x0, y0, z0))
+                    \<le> count_list (SST.eta_hat msst (fst qb, w) x) (Inl x0) * l"
+            by (simp add: count_alpha_hat_homU_eta_hat[OF bc_msst boundedness_l typed bc_type r_pair tail])
+        qed
+        have "(\<Sum>x\<in>UNIV. count_alpha (hat_homU (\<iota> B2 (Rep_alpha B2 (snd qb))) (SST.eta_hat msst (fst qb, w) x)) (Inl (x0, y0, z0)))
+            \<le> (\<Sum>x\<in>UNIV. count_list (SST.eta_hat msst (fst qb, w) x) (Inl x0) * l)"
+          by (simp add: body sum_mono)
+        also have "... = (\<Sum>x\<in>UNIV. count_list (SST.eta_hat msst (fst qb, w) x) (Inl x0)) * l"
+          by (metis (mono_tags, lifting) sum.cong sum_distrib_right)
+        also have "... = count_var (SST.eta_hat msst (fst qb, w)) x0 * l"
+          unfolding count_var_def by simp
+        also have "... \<le> k * l" proof -
+          have "bounded k (SST.eta_hat msst (fst qb, w))"
+            using bc_msst r_fst unfolding bounded_copy_SST_def by auto
+          then have "count_var (SST.eta_hat msst (fst qb, w)) x0 \<le> k"
+            by (simp add: bounded_def)
+          then show ?thesis by simp
+        qed
+        finally show ?thesis .
+      qed
+      finally show "?lhs \<le> k * l" .
+    qed
+  qed
+qed
+
+lemma "f (g x :: 'a list) = h (g x)"
+proof -
+  fix u
+  show "f u = h u" proof (induct "(g x)")
+
+  
 
 
 end
